src/impl/TLS13.Impl.Server.Driver.fsti
@@ -13,6 +13,8 @@ module CM = TLS13.Impl.ConnectionState.Model
 module CR = TLS13.Impl.ConnectionState.Repr
 module DL = TLS13.Impl.Server.Driver.Local
 module DN = TLS13.Impl.Server.Driver.Network
+module SQueries = TLS13.Impl.Server.CanonicalQueries
+module EP = TLS13.Impl.Server.Endpoint
 module Seq = FStar.Seq
 module SeqP = FStar.Seq.Properties
 module ST = TLS13.Impl.Server.Types
@@ -20,6 +22,7 @@ module SZ = FStar.SizeT
 module T = TLS13.Types
 module U16 = FStar.UInt16
 module U8 = FStar.UInt8
+module V = Pulse.Lib.Vec
 module SP = TLS13.Impl.Server.CanonicalProtocol
 
 val server_driver : Type0
@@ -34,6 +37,40 @@ val server_driver_canonical_progress
   (d: server_driver)
   (st: CS.connection_state)
   : slprop
+
+noextract
+val server_driver_endpoint_config
+  (d: server_driver)
+  : SQueries.server_next_local_action_config
+
+noextract
+val server_driver_endpoint_frame
+  (d: server_driver)
+  (network_app_out: array U8.t)
+  (network_app_out_len: SZ.t)
+  (local_payload: array U8.t)
+  (local_payload_len: SZ.t)
+  (local_app_out: array U8.t)
+  (local_app_out_len: SZ.t)
+  (certificate_chain_len: SZ.t)
+  (certificate_chain_len_proof:
+    (certificate_chain:Ghost.erased B.bytes ->
+      Ghost.erased
+        (SZ.v certificate_chain_len == B.length (Ghost.reveal certificate_chain))))
+  (certificate_chain_len_bound:
+    Ghost.erased
+      (SZ.v certificate_chain_len <= Bounds.max_server_certificate_chain_len))
+  (material_spec: Ghost.erased (b:B.bytes{B.length b == 64}))
+  (private_key: V.vec U8.t)
+  (material_deferred_ready:
+    (st:Ghost.erased CS.connection_state ->
+    action:SQueries.server_deferred_action ->
+      Ghost.erased
+        (SQueries.server_deferred_action_ready (Ghost.reveal st) action ==>
+         EP.server_endpoint_material_bytes_match_state
+           (Ghost.reveal material_spec)
+           (Ghost.reveal st))))
+  : EP.server_endpoint_frame
 
 noextract
 val server_driver_wire_logs_match
@@ -67,6 +104,20 @@ val server_driver_connected
   (credential_identity:CS.server_credential_identity)
   (received:B.bytes)
   (sent:B.bytes)
+  : slprop
+
+noextract
+val server_driver_endpoint_connected
+  (d:server_driver)
+  (cfg:SQueries.server_next_local_action_config)
+  (frame:EP.server_endpoint_frame)
+  (st:CS.connection_state)
+  (certificate_chain:B.bytes)
+  (credential_identity:CS.server_credential_identity)
+  (canonical_received:B.bytes)
+  (canonical_sent:B.bytes)
+  (transport_received:B.bytes)
+  (transport_sent:B.bytes)
   : slprop
 
 noextract
